

# Logic Practical Week 13

Question 3:

Show that the following propositional formulae are tautologies without using truth tables:

$$1. (\neg q \wedge (p \Rightarrow q)) \Rightarrow \neg q$$

$$2. ((p \vee q) \wedge \neg p) \Rightarrow q$$

$$1. (\neg q \wedge (p \Rightarrow q)) \Rightarrow \neg q$$

$  \begin{aligned}  &(\neg q \wedge (p \Rightarrow q)) \Rightarrow \neg q && \text{(Implication Law)} \\  &(\neg q \wedge (\neg p \vee q)) && \text{(Distribution Law)} \\  &(\neg q \wedge \neg p) \vee (\neg q \wedge q) && \text{(De Morgan's)} \\  &\quad \neg(q \vee p) \Rightarrow \neg q && \text{(Implication Law)} \\  &(q \vee p) \vee \neg q \\  &\quad 1 \quad \checkmark  \end{aligned}  $	$  \begin{aligned}  &((p \vee q) \wedge \neg p) \Rightarrow q \\  &(\neg p \wedge p) \vee (\neg p \wedge q) \\  &\quad (\neg p \wedge q) \Rightarrow q \\  &\quad \neg(\neg p \wedge q) \vee q \\  &\quad (p \vee \neg q) \vee q \\  &\quad 1 \quad \checkmark  \end{aligned}  $	$((p \vee q) \wedge \neg p) \Rightarrow q$
---	--	--

Question 4:

Show that  $(a \vee c) \wedge (b \Rightarrow c) \wedge (c \Rightarrow a)$  and  $(b \Rightarrow c) \wedge a$  are logically equivalent without using truth tables.

**Equation 1:**

$(a \vee c) \wedge (b \Rightarrow c) \wedge (c \Rightarrow a)$	(Implication Law)
$(a \vee c) \wedge (\neg b \vee c) \wedge (\neg c \vee a)$	(Commutativity)
$(a \vee c) \wedge (a \vee \neg c) \wedge (\neg b \vee c)$	(Distribution Law)
$(a \vee (c \wedge \neg c)) \wedge (\neg b \vee c)$	
$a \wedge (\neg b \vee c)$	

**Equation 2:**

$(b \Rightarrow c) \wedge a$	(Implication Law)
$(\neg b \vee c) \wedge a$	(Commutative Law)
$a \wedge (\neg b \vee c)$	

$\therefore \text{Equation 1} \equiv \text{Equation 2}$

Question 9: Conjunctive Normal Form

**Question 9: Conjunctive normal form**

Reduce the following formulae  $\varphi$  to conjunctive normal form without using truth tables.

$$1. ((p \wedge \neg q) \vee r) \Rightarrow (\neg p \wedge \neg r)$$

$$2. (p \wedge (q \Rightarrow r)) \Rightarrow s$$

$$3. (p_1 \wedge p_2) \vee (p_3 \wedge (p_4 \vee p_5))$$

$$1. ((p \wedge \neg q) \vee r) \Rightarrow (\neg p \wedge \neg r)$$

$$\begin{aligned}
 & ((p \wedge \neg q) \vee r) \Rightarrow (\neg p \wedge \neg r) && \text{(Implication Law)} \\
 & \neg((p \wedge \neg q) \vee r) \vee (\neg p \wedge \neg r) && \text{(De Morgan's)} \\
 & (\neg(p \wedge \neg q) \wedge \neg r) \vee (\neg p \wedge \neg r) && \text{(Distribution Law)} \\
 & \neg r \wedge (\neg p \vee (\neg(p \wedge \neg q))) && \text{(De Morgan's)} \\
 & \neg r \wedge (\neg p \vee (\neg p \vee q)) \\
 & \neg r \wedge (\neg p \vee q) \checkmark
 \end{aligned}$$

$$2. (p \wedge (q \Rightarrow r)) \Rightarrow s$$

$$\begin{aligned}
 & (p \wedge (q \Rightarrow r)) \Rightarrow s && \text{(Implication Law)} \\
 & \neg(p \wedge (q \Rightarrow r)) \vee s && \text{(Implication Law)} \\
 & \neg(p \wedge (\neg q \vee r)) \vee s && \text{(De Morgan's)} \\
 & (\neg p \vee \neg(\neg q \vee r)) \vee s && \text{(De Morgan's)} \\
 & (\neg p \vee (q \wedge \neg r)) \vee s && \text{(Distribution Law)} \\
 & ((\neg p \vee q) \wedge (\neg p \vee \neg r)) \vee s
 \end{aligned}$$

General Formula: (Distribution Law)

$$(A \wedge B) \vee C \equiv (C \vee A) \wedge (C \vee B)$$

Where  $A = (\neg p \vee q)$ ,  $B = (\neg p \vee \neg r)$ ,  $C = s$

Applying the General Formula:

$$\begin{aligned}
 & ((\neg p \vee q) \wedge (\neg p \vee \neg r)) \vee s \\
 & (s \vee (\neg p \vee q)) \wedge (s \vee (\neg p \vee \neg r)) \\
 & (s \vee \neg p \vee q) \wedge (s \vee \neg p \vee \neg r) \checkmark
 \end{aligned}$$